reduction

src/tm.lean
@@ -1,65 +1,476 @@
-import tactic
+import tactic data.vector.zip algebra.big_operators.basic algebra.big_operators.norm_num
+import vorspiel
+
+
+open_locale big_operators
 
 universes u v
 
 namespace turing_machine
 
-structure graph :=
-(vertices : Type u)
-(edge : Type)
-(map : edge → vertices → vertices → Prop)
-
-@[notation_class] class language (α : Type u) := (blank : α) (start : α)
-
-instance : language bool := ⟨ff, tt⟩
+inductive language (Γ : Type u)
+| blank : language
+| start : language
+| chr   : Γ → language
 
 notation `␣` := language.blank 
-notation `␤` := language.start 
+notation `␤` := language.start
+
+class state_lang (Q : Type u) :=
+(start : Q)
+(halt : Q)
+
+instance {Q R} [state_lang Q] [state_lang R] : state_lang (Q ⊕ R) := ⟨sum.inl state_lang.start, sum.inr state_lang.halt⟩
+
+end turing_machine
+
+def option.to_language {Γ : Type u} : option Γ → turing_machine.language Γ
+| none     := ␣
+| (some x) := turing_machine.language.chr x
+
+namespace turing_machine
+open state_lang
+
+namespace TM
+
+inductive deg 
+| stay  : deg
+| right : deg
+| left  : deg
+
+end TM
 
 class tape_class (α : Type u) := (input : α) (output : α)
 
 variables
-  (σ : Type) [language σ] -- 言語
-  (κ : Type) [inhabited κ] -- 状態
-  (η : Type) [tape_class η] -- ヘッド
-  (π : graph) -- グラフ
-  
-inductive word
-| mk : κ × (η → σ) → κ × (η → σ) × (η → π.edge) → word
+  (Γ : Type u) -- 言語
+  (Q : Type v) -- 状態
+  (ι : ℕ) -- テープの数
+
+inductive instruction
+| stay  : instruction
+| right : instruction
+| left  : instruction
+
+@[simp] def instruction.apply : instruction → ℕ → ℕ
+| instruction.stay  ι := ι
+| instruction.right ι := ι + 1
+| instruction.left  ι := ι - 1
+
+structure word :=
+(cond : Q × vector Γ ι)
+(cons : Q × vector (Γ × instruction) ι)
 
 infix ` ▷ `:80 := word.mk
 
+structure line :=
+(tape : ℕ → Γ)
+(head : ℕ)
+
+@[ext] lemma line.ext (l₁ l₂ : line Γ) (et : l₁.tape = l₂.tape) (eh : l₁.head = l₂.head) : l₁ = l₂ :=
+by { rcases l₁; rcases l₂, simp at et eh, simp[eh, et] }
+
 structure model :=
-(tape : η → π.vertices → σ)
-(head : η → π.vertices)
-(state : κ)
+(state : Q) 
+(lines : vector (line Γ) ι)
 
-variables {σ κ η π} (p : set (word σ κ η π))
 
-def model.read (m : model σ κ η π) (i : η) : σ :=
-m.tape i (m.head i)
+abbreviation sentence := set (word Γ Q ι)
 
-inductive reduction : model σ κ η π → model σ κ η π → Prop
-| reduct : ∀ {x : η → π.edge} (m₀ m₁ : model σ κ η π), 
-    (∀ i : η, π.map (x i) (m₀.head i) (m₁.head i)) →
-     ⟨m₀.state, m₀.read⟩ ▷ ⟨m₁.state, λ i, m₁.tape i (m₀.head i), x⟩ ∈ p → reduction m₀ m₁
+variables {Γ Q ι}
+
+namespace model
+variables (σ : sentence Γ Q ι)
+
+@[ext] lemma ext : ∀ {m₁ m₂ : model Γ Q ι}
+  (input : m₁.lines = m₂.lines)
+  (state : m₁.state = m₂.state), m₁ = m₂
+| ⟨q₁, L₁⟩ ⟨q₂, L₂⟩ tape state :=
+  by { simp, split, { exact state }, { funext, exact tape }  }
+
+def read (m : model Γ Q ι) : vector Γ ι := m.lines.map (λ l, l.1 l.2)
+
+def snapshot (m : model Γ Q ι) : Q × vector Γ ι := ⟨m.state, m.lines.map (λ ⟨T, n⟩, T n)⟩
+
+def reduct (q : Q) (z : vector (Γ × instruction) ι) : model Γ Q ι → model Γ Q ι
+| ⟨_, L⟩ :=
+  { lines := @vector.zip_with (line Γ) (Γ × instruction) (line Γ) ι
+      (λ ⟨T, h⟩ ⟨x, i⟩, ⟨λ n, if n = h then x else T n, i.apply h⟩) L z,
+    state := q }
+
+@[simp] lemma reduct_head (m : model Γ Q ι) (q : Q) (z : vector (Γ × instruction) ι) :
+  (reduct q z m).state = q := by cases m; simp[reduct]
+
+lemma reduct_lines_nth (m : model Γ Q ι) (q : Q) (z : vector (Γ × instruction) ι) (i : fin ι) :
+  (reduct q z m).lines.nth i = ⟨λ n, if n = (m.lines.nth i).2 then (z.nth i).1 else (m.lines.nth i).1 n, (z.nth i).2.apply (m.lines.nth i).2⟩ :=
+by { rcases m with ⟨_, L⟩, rcases eL : L.nth i with ⟨T, h⟩, rcases ez: z.nth i with ⟨x, ins⟩, simp[eL, ez, reduct] }
+
+
+inductive reduction : model Γ Q ι → model Γ Q ι → Prop
+| intro : ∀ (m : model Γ Q ι) (q : Q) (z : vector (Γ × instruction) ι),
+    ⟨m.state, m.read⟩ ▷ ⟨q, z⟩ ∈ σ → reduction m (reduct q z m)
   
-notation m₀ ` ⟶¹[`:60  p `]` :0 m₁ := reduction p m₀ m₁ 
+notation m₀ ` ⟶¹[`:60  σ `] ` :0 m₁ := reduction σ m₀ m₁ 
 
-def is_halt (m : model σ κ η π) : Prop := ∀ m', ¬m ⟶¹[p] m'
+def is_halt (m : model Γ Q ι) : Prop := ∀ m', ¬m ⟶¹[σ] m'
 
-inductive time_bound_reduction : ℕ → model σ κ η π → model σ κ η π → Prop
-| symm : ∀ m, time_bound_reduction 0 m m
-| succ : ∀ {n m₀ m₁ m₂}, time_bound_reduction n m₀ m₁ → (m₁ ⟶¹[p] m₂) → time_bound_reduction (n + 1) m₀ m₂
+inductive time_reductions : ℕ → model Γ Q ι → model Γ Q ι → Prop
+| zero : ∀ m, time_reductions 0 m m
+| succ : ∀ {ι m₀ m₁ m₂}, time_reductions ι m₀ m₁ → (m₁ ⟶¹[σ] m₂) → time_reductions ι.succ m₀ m₂
 
-notation m₀ ` ⟶^(` n `)[`:60  p `]` :0 m₁ := time_bound_reduction p n m₀ m₁ 
+attribute [simp] time_reductions.zero
 
-def termination (m₀ m₁ : model σ κ η π) : Prop := is_halt p m₁ ∧ (∃ n : ℕ, m₀ ⟶^(n)[p] m₁)
+notation m₀ ` ⟶^(`:80 s `)[`:80  σ `] ` :0 m₁ := time_reductions σ s m₀ m₁ 
 
-notation m₀ ` ⟶ᵗ ` m₁ := termination m₀ m₁
+def time_bounded_reductions (s : ℕ) (m m' : model Γ Q ι) : Prop := ∃ s' ≤ s, m ⟶^(s')[σ] m'
+notation m₀ ` ⟶^(≤ ` s `)[`:80  σ `] ` :0 m₁ := time_bounded_reductions σ s m₀ m₁ 
 
-def initial (l : π.vertices → σ) : model σ κ η π :=
-  { tape := λ i x, by {  },
-    head := λ i, {  } }
+def time_bounded_reductions_halt (s : ℕ) (m m' : model Γ Q ι) : Prop := is_halt σ m' ∧ ∃ s' ≤ s, m ⟶^(s')[σ] m'
+notation m₀ ` ⟶^(≤ ` s `)[`:80  σ `]↓ ` :0 m₁ := time_bounded_reductions_halt σ s m₀ m₁ 
+
+def reductions (m m' : model Γ Q ι) : Prop := ∃ s : ℕ, m ⟶^(s)[σ] m' 
+
+notation m₀ ` ⟶*[`:80  σ `] ` :0 m₁ := reductions σ m₀ m₁ 
+
+def converge (m₀ m₁ : model Γ Q ι) : Prop := is_halt σ m₁ ∧ (m₀ ⟶*[σ] m₁)
+
+notation m₀ ` ⟶ᵗ[`:80 σ `] ` :0 m₁ := converge m₀ m₁
+
+end model
+
+variables {Γ Q ι} 
+def sentence.deterministic (σ : sentence Γ Q ι) : Prop := ∀ q q₁ q₂, q ▷ q₁ ∈ σ → q ▷ q₂ ∈ σ → q₁ = q₂
+
+def sentence.proper [state_lang Q] (σ : sentence Γ Q ι) : Prop :=
+  ∀ w₁ w₂, w₁ ▷ w₂ ∈ σ → w₁.1 ≠ state_lang.halt ∧ w₂.1 ≠ state_lang.start
+
+namespace sentence
+
+namespace deterministic
+variables {σ : sentence Γ Q ι} {m₁ m₂ : model Γ Q ι}
+
+lemma reduction (d : deterministic σ) {m m₁ m₂}
+  (h₁ : m ⟶¹[σ] m₁) (h₂ : m ⟶¹[σ] m₂) : m₁ = m₂ :=
+begin
+  rcases h₁ with ⟨_, q₁, z₁, w₁⟩,
+  rcases h₂ with ⟨_, q₂, z₂, w₂⟩,
+  have : q₁ = q₂ ∧ z₁ = z₂, by simpa using d _ _ _ w₁ w₂,
+  rcases this with ⟨rfl, rfl, rfl⟩,
+  refl
+end
+
+lemma time_reductions (d : deterministic σ) {m m₁ m₂} {s} (h₁ : m ⟶^(s)[σ] m₁) (h₂ : m ⟶^(s)[σ] m₂) :
+  m₁ = m₂ :=
+begin
+  induction s with s IH generalizing m₁ m₂,
+  { rcases h₁, rcases h₂, refl },
+  { rcases h₁ with (_ | ⟨_, _, m₁₁, _, h_₁₁, h₁₁_₁⟩),
+    rcases h₂ with (_ | ⟨_, _, m₂₁, _, h_₂₁, h₂₁_₂⟩),
+    have : m₁₁ = m₂₁, from IH h_₁₁ h_₂₁, rcases this with rfl,
+    exact reduction @d h₁₁_₁ h₂₁_₂ }
+end
+
+end deterministic
+
+end sentence
+
+namespace model
+open sentence sentence.deterministic
+variables {m₁ m₂ m₃ : model Γ Q ι} {σ : sentence Γ Q ι}
+
+@[simp] lemma time_bounded_reductions.refl {s} : m₁ ⟶^(≤ s)[σ] m₁ :=
+⟨0, zero_le s, time_reductions.zero m₁⟩
+
+lemma time_bounded_reductions.of_le {s₁ s₂} (h : m₁ ⟶^(≤ s₁)[σ] m₂) (le : s₁ ≤ s₂) :
+  m₁ ⟶^(≤ s₂)[σ] m₂ := 
+by rcases h with ⟨s, le_s, h⟩; refine ⟨s, le_trans le_s le, h⟩
+
+lemma time_reductions.add {s₁ s₂} (h₁ : m₁ ⟶^(s₁)[σ] m₂) (h₂ : m₂ ⟶^(s₂)[σ] m₃) :
+  m₁ ⟶^(s₁ + s₂)[σ] m₃ :=
+begin
+  induction s₂ with s₂ IH generalizing s₁ m₁ m₂ m₃,
+  { rcases h₂, exact h₁ },
+  { rcases h₂ with (_| ⟨_, _, m₂₁, _, h₂_₂₁, h₂₁_₃⟩),
+  simpa using (IH h₁ h₂_₂₁).succ h₂₁_₃ }
+end
+
+lemma time_bounded_reductions.add {s₁ s₂} (h₁ : m₁ ⟶^(≤ s₁)[σ] m₂) (h₂ : m₂ ⟶^(≤ s₂)[σ] m₃) :
+  m₁ ⟶^(≤ s₁ + s₂)[σ] m₃ :=
+begin
+  rcases h₁ with ⟨t₁, le₁, h₁⟩,
+  rcases h₂ with ⟨t₂, le₂, h₂⟩,
+  refine ⟨t₁ + t₂, add_le_add le₁ le₂, h₁.add h₂⟩,
+end
+
+lemma time_bounded_reductions.sum {m : ℕ → model Γ Q ι} {s : ℕ → ℕ}
+  (h : ∀ k, m k ⟶^(≤ s k)[σ] m (k + 1)) (k : ℕ) : (m 0) ⟶^(≤ ∑ i in finset.range k, s i)[σ] (m k) :=
+by { induction k with k IH, { simp }, { simpa[finset.sum_range_succ] using IH.add (h k) } }
+
+lemma reduction.of_ss (r : m₁ ⟶¹[σ] m₂) {τ : sentence Γ Q ι} (ss : σ ⊆ τ) : m₁ ⟶¹[τ] m₂ :=
+by { rcases r with ⟨_, q, z, mem⟩, refine ⟨_, _, _, _⟩, exact ss mem }
+
+lemma time_reductions.of_ss {n} (r : m₁ ⟶^(n)[σ] m₂) {τ : sentence Γ Q ι} (ss : σ ⊆ τ) : m₁ ⟶^(n)[τ] m₂ :=
+by { induction n with n IH generalizing m₂, { rcases r, simp },
+     { rcases r with (_ | ⟨_, _, m₁₁, _, r₁_₁₁, r₁₁_₂⟩), exact (IH r₁_₁₁).succ (r₁₁_₂.of_ss ss) } }
+
+lemma time_bounded_reductions.of_ss {k} (r : m₁ ⟶^(≤ k)[σ] m₂) {τ : sentence Γ Q ι} (ss : σ ⊆ τ) : m₁ ⟶^(≤ k)[τ] m₂ :=
+by { rcases r with ⟨n, le, r⟩, refine ⟨n, le, r.of_ss ss⟩ }
+
+section
+variables {R : Type v} (f : Q → R)
+
+@[simp] def map_q : model Γ Q ι → model Γ R ι
+| ⟨q, L⟩ := ⟨f q, L⟩
+
+instance [has_coe Q R] : has_coe (model Γ Q ι) (model Γ R ι) := ⟨λ m, m.map_q coe⟩ 
+
+@[simp] def word.map_q : word Γ Q ι → word Γ R ι
+| (⟨q, w⟩ ▷ ⟨q', w'⟩) :=  ⟨f q, w⟩ ▷ ⟨f q', w'⟩
+
+variables (m m' : model Γ Q ι) {f}
+
+@[simp] lemma map_q_lines (m : model Γ Q ι) : (m.map_q f).lines = m.lines := by cases m; simp
+
+@[simp] lemma map_q_state (m : model Γ Q ι) : (m.map_q f).state = f m.state := by cases m; simp
+
+@[simp] lemma map_q_reduct (q : Q) (z : vector (Γ × instruction) ι) :
+  (reduct q z m).map_q f = reduct (f q) z (m.map_q f) := by cases m; simp[reduct]
+
+@[simp] lemma map_q_snapshot : (m.map_q f).read = m.read :=  by cases m; simp[read]
+
+variables (f)
+
+lemma reduction.map_q (h : m₁ ⟶¹[σ] m₂) (f : Q → R) : m₁.map_q f ⟶¹[word.map_q f '' σ] m₂.map_q f :=
+by { rcases h with ⟨_, q, w, mem⟩, simp, refine ⟨_, _, _, _⟩, simp, refine ⟨_, mem, by simp⟩ }
+
+lemma time_reductions.map_q {n} (h : m₁ ⟶^(n)[σ] m₂) (f : Q → R) : m₁.map_q f ⟶^(n)[word.map_q f '' σ] m₂.map_q f :=
+by { induction n with n IH generalizing m₂, { rcases h, simp },
+     { rcases h with (_ | ⟨_, _, m₁₁, _, r₁_₁₁, r₁₁_₂⟩), refine (IH r₁_₁₁).succ (r₁₁_₂.map_q f) } }
+
+lemma time_bounded_reduction.map_q {k} (h : m₁ ⟶^(≤ k)[σ] m₂) (f : Q → R) : m₁.map_q f ⟶^(≤ k)[word.map_q f '' σ] m₂.map_q f :=
+by { rcases h with ⟨n, le, r⟩, refine ⟨n, le, r.map_q f⟩ }
+
+variables {f}
+
+lemma deterministic.map_q (inj : function.injective f) (d : deterministic σ) : deterministic (word.map_q f '' σ) :=
+begin
+  rintros ⟨r, w⟩ ⟨r₁, w₁⟩ ⟨r₂, w₂⟩ h₁ h₂,
+  rcases h₁ with ⟨⟨⟨q, w'⟩, ⟨q₁, w₁'⟩⟩, mem₁, eq₁⟩,
+  have : f q = r ∧ w = w' ∧ f q₁ = r₁ ∧ w₁ = w₁', { simp at eq₁, simp[eq₁] },
+  rcases this with ⟨rfl, rfl, rfl, rfl⟩,
+  rcases h₂ with ⟨⟨⟨q', w'⟩, ⟨q₂, w₂'⟩⟩, mem₂, eq₂⟩,
+  have : f q' = f q ∧ w = w' ∧ f q₂ = r₂ ∧ w₂ = w₂', { simp at eq₂, simp[eq₂] },
+  rcases this with ⟨eq, rfl, rfl, rfl⟩,
+  have : q = q', from (inj eq).symm, rcases this with rfl,
+  have : q₁ = q₂ ∧ w₁ = w₂, by simpa using d _ _ _ mem₁ mem₂,
+  simp[this] 
+end
+
+end
+
+variables {R : Type v}
+
+inductive sentence.fix_q (q₁ q₂ : Q) : sentence Γ Q ι
+| intro : ∀ v : vector Γ ι, sentence.fix_q ((q₁, v) ▷ (q₂, v.map (λ x, (x, instruction.stay))))
+
+@[simp] lemma sentence.fix_q_mem (q₁ q₂ : Q) (v : vector Γ ι) :
+   ((q₁, v) ▷ (q₂, v.map (λ x, (x, instruction.stay)))) ∈ (sentence.fix_q q₁ q₂ : sentence Γ Q ι) :=
+sentence.fix_q.intro v
+
+lemma sentence.fix_q.deterministic (q₁ q₂ : Q) : deterministic (sentence.fix_q q₁ q₂ : sentence Γ Q ι) :=
+by { rintros w w₁ w₂ h₁ h₂, rcases h₁, rcases h₂, simp }
+
+lemma sentence.fix_q_reduction (q₁ q₂ : Q) (L : vector (line Γ) ι) : ⟨q₁, L⟩ ⟶¹[sentence.fix_q q₁ q₂] ⟨q₂, L⟩ :=
+begin
+  let v := (⟨q₁, L⟩ : model Γ Q ι).read,
+  let z := vector.map (λ (x : Γ), (x, instruction.stay)) v,
+  suffices : ⟨q₁, L⟩ ⟶¹[fix_q q₁ q₂] reduct q₂ z ⟨q₁, L⟩,
+  { have e: (⟨q₂, L⟩ : model Γ Q ι) = reduct q₂ z ⟨q₁, L⟩,
+    { ext; simp[reduct_lines_nth, v, read], by_cases e : x = (L.nth m).head; simp[e] },
+    simpa[e] using this },
+  have : (q₁, v) ▷ (q₂, z) ∈ fix_q q₁ q₂, from sentence.fix_q_mem q₁ q₂ v,
+  refine reduction.intro ⟨q₁, L⟩ q₂ z this
+end
+
+def deterministic.union {σ τ : sentence Γ Q ι} (dσ : deterministic σ) (dτ : deterministic τ)
+  (h : ∀ (w₁ w₂ : word Γ Q ι), w₁ ∈ σ → w₂ ∈ τ → w₁.cond = w₂.cond → w₁.cons = w₂.cons) : deterministic (σ ∪ τ) :=
+begin
+    rintros w w₁ w₂ h₁ h₂,
+   rcases h₁,
+   { rcases h₂, { exact dσ _ _ _ h₁ h₂ }, { simpa using h _ _ h₁ h₂ (by simp) } },
+   { rcases h₂, { simpa using (h _ _ h₂ h₁ (by simp)).symm }, { exact dτ _ _ _ h₁ h₂ } }
+end
+
+variables [state_lang Q] [state_lang R]
+
+def sentence.dsum (σ : sentence Γ Q ι) (τ : sentence Γ R ι) : sentence Γ (Q ⊕ R) ι :=
+(word.map_q sum.inl '' σ) ∪ (word.map_q sum.inr '' τ) ∪ (sentence.fix_q (sum.inl (halt : Q)) (sum.inr (start : R)))
+
+infix ` ⨁ `:80 := sentence.dsum
+
+lemma sentence.dsum.deterministic {σ : sentence Γ Q ι} {τ : sentence Γ R ι}
+  (proper : proper σ) (d₁ : deterministic σ) (d₂ : deterministic τ) : deterministic (σ ⨁ τ) :=
+begin
+  have : deterministic ((word.map_q sum.inl '' σ) ∪ (word.map_q sum.inr '' τ) : sentence Γ (Q ⊕ R) ι),
+  { refine deterministic.union (deterministic.map_q (sum.inl_injective) d₁) (deterministic.map_q (sum.inr_injective) d₂) _,
+    simp, rintros ⟨v₁, w₁⟩ ⟨v₂, w₂⟩ ⟨⟨q₁, u₁⟩, q'₁, u'₁⟩ mem₁,
+    simp, rintros rfl rfl ⟨⟨q₂, u₂⟩, q'₂, u'₂⟩ mem₂,
+    simp, rintros rfl rfl, simp },
+  refine deterministic.union this (sentence.fix_q.deterministic _ _) _,
+  rintros w₁ w₂ (⟨⟨⟨q, w⟩, ⟨q', w'⟩⟩, mem, rfl⟩ | ⟨⟨⟨q, w⟩, ⟨q', w'⟩⟩, mem, rfl⟩) ⟨_, _⟩,
+  { simp, rintros rfl, exfalso, simpa using proper _ _ mem },
+  { simp }
+end
+
+lemma time_reductions.dsum_aux  {σ : sentence Γ Q ι} {τ : sentence Γ R ι} {n₁ n₂ : ℕ} {m₁ : model Γ Q ι} {L : vector (line Γ) ι} {m₂ : model Γ R ι}
+  (h₁ : m₁ ⟶^(n₁)[σ] ⟨halt, L⟩) (h₂ : ⟨start, L⟩ ⟶^(n₂)[τ] m₂) :
+  m₁.map_q sum.inl ⟶^(n₁ + n₂ + 1)[σ ⨁ τ] m₂.map_q sum.inr :=
+begin
+  have h₁ : m₁.map_q sum.inl ⟶^(n₁)[σ ⨁ τ] ⟨sum.inl halt, L⟩,
+  { have : m₁.map_q sum.inl ⟶^(n₁)[word.map_q (sum.inl : Q → Q ⊕ R) '' σ] ⟨sum.inl halt, L⟩,
+      by simpa using h₁.map_q (sum.inl : Q → Q ⊕ R),
+    refine this.of_ss (by { simp[sentence.dsum, -set.image_subset_iff], 
+      refine set.subset_union_of_subset_left (set.subset_union_left _ _) _ }) },
+  have h : ⟨sum.inl halt, L⟩ ⟶¹[σ ⨁ τ] ⟨sum.inr start, L⟩,
+  { have : ⟨sum.inl halt, L⟩ ⟶¹[sentence.fix_q (sum.inl (halt : Q)) (sum.inr (start : R))] ⟨sum.inr start, L⟩,
+      from sentence.fix_q_reduction (sum.inl halt) (sum.inr start) L,
+    refine this.of_ss (by simp[sentence.dsum, -set.image_subset_iff]) },
+  have h₂ :  ⟨sum.inr start, L⟩ ⟶^(n₂)[σ ⨁ τ] m₂.map_q sum.inr,
+  { have : ⟨sum.inr start, L⟩ ⟶^(n₂)[word.map_q (sum.inr : R → Q ⊕ R) '' τ] m₂.map_q sum.inr,
+      by simpa using h₂.map_q (sum.inr : R → Q ⊕ R),
+    refine this.of_ss (by { simp[sentence.dsum, -set.image_subset_iff], 
+      refine set.subset_union_of_subset_left (set.subset_union_right _ _) _ }) },
+  simpa[show n₁.succ + n₂ = n₁ + n₂ + 1, by omega] using (h₁.succ h).add h₂,
+end
+
+lemma time_reductions.dsum  {σ : sentence Γ Q ι} {τ : sentence Γ R ι} {n₁ n₂ : ℕ} {L₁ L₂ L₃ : vector (line Γ) ι}
+  (h₁ : ⟨start, L₁⟩ ⟶^(n₁)[σ] ⟨halt, L₂⟩) (h₂ : ⟨start, L₂⟩ ⟶^(n₂)[τ] ⟨halt, L₃⟩) :
+  ⟨start, L₁⟩ ⟶^(n₁ + n₂ + 1)[σ ⨁ τ] ⟨halt, L₃⟩ :=
+time_reductions.dsum_aux h₁ h₂
+
+
+lemma reduction_of_fn 
+
+
+end model
+/--/
+variables {Γ Q ι} 
+def deterministic (σ : sentence Γ Q ι) : Prop := ∀ {q q₁ q₂}, q ▷ q₁ ∈ σ → q ▷ q₂ ∈ σ → q₁ = q₂
+
+namespace deterministic
+variables {σ : sentence Γ Q ι} {m₁ m₂ : model Γ Q ι}
+
+lemma reduction (d : deterministic σ) {m m₁ m₂}
+  (h₁ : m ⟶¹[σ] m₁) (h₂ : m ⟶¹[σ] m₂) : m₁ = m₂ :=
+begin
+  rcases h₁ with ⟨_, q₁, z₁, w₁⟩,
+  rcases h₂ with ⟨_, q₂, z₂, w₂⟩,
+  have : q₁ = q₂ ∧ z₁ = z₂, by simpa using d w₁ w₂,
+  rcases this with ⟨rfl, rfl, rfl⟩,
+  refl
+end
+
+lemma time_reductions (d : deterministic σ) {m m₁ m₂} {s} (h₁ : m ⟶^(s)[σ] m₁) (h₂ : m ⟶^(s)[σ] m₂) :
+  m₁ = m₂ :=
+begin
+  induction s with s IH generalizing m₁ m₂,
+  { rcases h₁, rcases h₂, refl },
+  { rcases h₁ with (_ | ⟨_, _, m₁₁, _, h_₁₁, h₁₁_₁⟩),
+    rcases h₂ with (_ | ⟨_, _, m₂₁, _, h_₂₁, h₂₁_₂⟩),
+    have : m₁₁ = m₂₁, from IH h_₁₁ h_₂₁, rcases this with rfl,
+    exact reduction @d h₁₁_₁ h₂₁_₂ }
+end
+
+end deterministic
+
+namespace TM
+variables [state Q] 
+
+instance : inhabited (tape (language Γ)) := ⟨⟨λ n, match n with | 0 := ␤ | (n + 1) := ␣ end, 0⟩⟩
+
+@[simp] lemma tape.default_head : (default : tape (language Γ)).head = 0 := rfl
+
+@[simp] lemma tape.default_tape_0 : (default : tape (language Γ)).tape 0 = ␤ := rfl
+
+@[simp] lemma tape.default_tape_gt0 {n} (h : n > 0) : (default : tape (language Γ)).tape n = ␣ :=
+by { cases n, { simp at h, contradiction }, { refl } }
+
+instance : inhabited (model (language Γ) Q ι) := ⟨⟨vector.repeat default ι, state.start⟩⟩
+
+@[simp] lemma model.default_state : (default : model (language Γ) Q ι).state = state.start := rfl
+
+@[simp] lemma model.default_lines : (default : model (language Γ) Q ι).lines = vector.repeat default ι := rfl
+
+def tape_of (x : list Γ) : ℕ → language Γ
+| 0       := ␤
+| (n + 1) := if h : n < x.length then language.chr (x.nth_le n h) else ␣
+
+-- ␤ x₁ x₂ ... xₙ ␣ ␣ ␣ ...
+
+@[simp] lemma tape_of_of_zero {x : list Γ} : tape_of x 0 = ␤ := by simp[tape_of]
+
+@[simp] lemma tape_of_of_lt {n} {x : list Γ} (gt : n > 0) (le : n ≤ x.length) :
+  tape_of x n = language.chr (x.nth_le (n - 1) (by { cases n, { simp at gt, contradiction }, { simpa using nat.succ_le_iff.mp le} })) :=
+by { cases n, { simp at gt, contradiction },
+     { simp[tape_of, show n < x.length, from nat.succ_le_iff.mp le] } }
+
+@[simp] lemma tape_of_list_of_ge {n} {x : list Γ} (h : n ≥ x.length + 1) : tape_of x n = ␣ :=
+by { cases n, { simp at h, contradiction },
+     { simp[tape_of], have : n ≥ x.length, exact nat.succ_le_succ_iff.mp h, exact nat.le_lt_antisymm this } }
+
+structure time_bounded_computable_by_NDTM (f : list Γ → list Γ) (T : ℕ → ℕ) :=
+(Q : Type*)
+(Q_fin : finite Q)
+(Q_state : state Q)
+(σ : sentence (language Γ) Q ι.succ.succ)
+(reduction : ∀ (X : list Γ), 
+  ⟨⟨tape_of X, 0⟩ ::ᵥ vector.repeat default ι.succ, state.start⟩ ⟶^(≤ T X.length)[σ]↓
+  ⟨vector.concat (vector.repeat default ι.succ) ⟨tape_of (f X), 0⟩, state.halt⟩)
+
+structure time_bounded_computable_by_TM (f : list Γ → list Γ) (T : ℕ → ℕ) :=
+(Q : Type*)
+(Q_fin : finite Q)
+(Q_state : state Q)
+(σ : sentence (language Γ) Q ι.succ.succ)
+(deterministic : deterministic σ)
+(reduction : ∀ (X : list Γ), 
+  ⟨⟨tape_of X, 0⟩ ::ᵥ vector.repeat default ι.succ, state.start⟩ ⟶^(≤ T X.length)[σ]↓
+  ⟨vector.concat (vector.repeat default ι.succ) ⟨tape_of (f X), 0⟩, state.halt⟩)
+
+
+
+
+variables {σ : sentence (language Γ) Q ι.succ}
+/--/
+
+
+
+structure time_bounded_computable_by_TM (f : list Γ → list Γ) (T : ℕ → ℕ) :=
+(Q : Type*)
+(Q_fin : finite Q)
+(Q_inhabited : inhabited Q)
+(σ : sentence (language Γ) Q ι.succ)
+(deterministic : deterministic σ)
+(reduction : ∀ (X : list Γ), encode X ⟶^(≤ T X.length)[σ]↓ encode (f X))
+
+def time_bounded_computable_by_TM (f : list Γ → list Γ) (T : ℕ → ℕ) : Prop :=
+  ∃ (c : ℕ) (Q : Type*) [fintype Q] (σ : sentence (language Γ) (state Q) (indexical empty) TM.tape)
+  deterministic σ ∧
+  ∀ (X : list Γ), ∃ (m : model (language Γ) (state Q) (indexical empty) TM.tape),
+  is_terminal (f X) m ∧ (initial X ⟶^(≤ c * T X.length)[σ]↓ m)
+
+lemma constant_computable_by_c : time_bounded_computable_by_TM (λ x : list bool, []) (λ ι, 0) :=
+begin
+  refine ⟨1, empty, fintype_of_option, ∅, by { intros _, simp }, λ X, _⟩,
+  simp, refine ⟨_, 0, by refl, _⟩,
+  { intros _ h,
+    exfalso,
+    rcases h with ⟨_, _, _, _, _, h⟩,
+    exact h },
+  {  }
+end
+
+end TM
 
 end turing_machine
+8
