src/vorspiel.lean
@@ -1,0 +1,17 @@
+import tactic data.vector data.vector.zip 
+
+universes u v
+
+def vorspiel : ℕ := 9
+
+namespace vector
+variables {α : Type u} {n : ℕ}
+
+def concat : vector α n → α → vector α n.succ
+| ⟨l, h⟩ a := ⟨l.concat a, by simp[h]⟩
+
+
+
+end vector
+
+#check vector.concat
